Printing.thy
@@ -2,6 +2,7 @@ theory Printing
   imports "02Typed/Typechecking" "03Debruijn/NameRemoval" "05Closure/ClosureConversion" 
     "06TreeCode/TreeCodeConversion" "07TailCall/TailCallOptimization" "08FlatCode/CodeFlattening" 
     "09HeapMemory/HeapConversion" "10ChainedEnvironment/Chaining" "11FlatMemory/MemoryFlattening"
+    "14MachineCode/Disassemble" 
 begin
 
 function string_of_nat :: "nat \<Rightarrow> string" where
@@ -53,9 +54,14 @@ primrec print_ceclosure :: "ceclosure \<Rightarrow> string" where
   "print_ceclosure (CEConst k) = string_of_nat k"
 | "print_ceclosure (CELam cs pc) = ''<fun>''"
 
-fun print_uclosure :: "(nat \<Rightarrow> nat) \<Rightarrow> nat \<Rightarrow> string" where
-  "print_uclosure h p = (case h p of
+fun print_uval :: "(nat \<Rightarrow> nat) \<Rightarrow> nat \<Rightarrow> string" where
+  "print_uval h p = (case h p of
       0 \<Rightarrow> string_of_nat (h (Suc p))
+    | Suc x \<Rightarrow> ''<fun>'')"
+
+fun print_mval :: "(nat \<Rightarrow> nat) \<Rightarrow> nat \<Rightarrow> string" where
+  "print_mval m p = (case m p of
+      0 \<Rightarrow> string_of_nat (m (4 + p))
     | Suc x \<Rightarrow> ''<fun>'')"
 
 lemma [simp]: "valt e \<Longrightarrow> print_texpr e = print_nexpr (erase e)" 
@@ -82,11 +88,15 @@ lemma [simp]: "print_bclosure c = print_tco_closure (unflatten_closure cd c)"
 lemma [simp]: "print_hclosure (hlookup h x) = print_bclosure (unheap_closure h x)"
   by (cases "hlookup h x") simp_all
 
-lemma print_ce [simp]: "print_ceclosure (hlookup h x) = 
-    print_hclosure (hlookup (unchain_heap h env) x)"
+lemma print_ce [simp]: "hcontains h x \<Longrightarrow> 
+    print_ceclosure (hlookup h x) = print_hclosure (hlookup (unchain_heap h env) x)"
   by (cases "hlookup h x") simp_all
 
-lemma print_u [simp]: "print_uclosure h p = print_ceclosure (get_closure (H h hp) p)"
+lemma print_u [simp]: "print_uval h p = print_ceclosure (get_closure (H h hp) p)"
   by (cases "h p") simp_all
+
+lemma print_m [simp]: "unmap_mem p = (a, b) \<Longrightarrow> 
+    print_mval (uncurry mem \<circ> unmap_mem) p = print_uval (mem a) b" 
+  by (auto split: nat.splits)
 
 end
